coq/common/lemmas/merge/cancl.v
@@ -11,7 +11,82 @@ Require Import common.defs.obj.
 
 (* Cancellativity: If Δ₁ ⋈ Δ₂ = Δ₁ ⋈ Δ₂', then Δ₂ = Δ₂' *)
 
+
+
+Lemma cx_eq_cons_refl :
+  forall {N : nat} (delta : lctx N) (obj : obj) (tp : tp.tp) (alpha : lin_aff.mult),
+    cx_eq delta delta ->
+    cx_eq (cons N delta obj tp alpha) (cons N delta obj tp alpha).
+Proof.
+  intros N delta obj tp alpha H_cx_eq.
+  inversion H_cx_eq; subst.
+  constructor.
+Qed.
+
+
+
 Lemma merge_cancl :
+  forall {N : nat} (psi : ctx) (delta delta1 delta2 delta2' : lctx N),
+    merge delta1 delta2 delta ->
+    merge delta1 delta2' delta ->
+    cx_eq delta2 delta2'.
+Proof.
+  intros N psi delta delta1 delta2 delta2' H_merge1 H_merge2.
+  generalize dependent delta2'.
+  induction H_merge1 as [| N delta1 delta2 delta obj tp alpha1 alpha2 alpha H_merge1 IH_merge H_mult].
+  - (* Base case *)
+    intros delta2' H_merge2.
+    dependent destruction H_merge2.
+    apply cx_refl.
+  - (* Inductive case *)
+    intros delta2' H_merge2.
+    dependent destruction H_merge2.
+    (* Use IH_merge to prove subcontext equality *)
+    specialize (IH_merge delta3 H_merge2).
+    inversion IH_merge; subst.
+    (* apply cx_eq_cons_refl. *)
+    Abort.
+
+(* Qed. *)
+
+
+
+Lemma merge_cancl :
+  forall {N : nat} (psi : ctx) (delta delta1 delta2 delta2' : lctx N),
+    merge delta1 delta2 delta ->
+    merge delta1 delta2' delta ->
+    cx_eq delta2 delta2'.
+Proof.
+  intros N psi delta delta1 delta2 delta2' H_merge1 H_merge2.
+  generalize dependent delta2'.
+  induction H_merge1 as [| N delta1 delta2 delta obj tp alpha1 alpha2 alpha H_merge1 IH_merge H_mult].
+  - (* Base case *)
+    intros delta2' H_merge2.
+    dependent destruction H_merge2.
+    apply cx_refl.
+  - (* Inductive case *)
+    intros delta2' H_merge2.
+    dependent destruction H_merge2.
+    (* Use IH_merge to prove subcontext equality *)
+    specialize (IH_merge delta3 H_merge2).
+    inversion IH_merge; subst.
+    (* Use mult_op_cancellation to align multiplicities *)
+    assert (alpha3 = tp) as H_alpha_eq.
+    Abort.
+(* Qed. *)
+
+    (* Prove multiplicities align *)
+    (* assert (alpha2 = alpha3). *)
+
+    (* Conclude cx_eq for the extended contexts *)
+    (* constructor. *)
+
+
+
+
+
+
+Lemma merge_cancl' :
   forall {N : nat} (delta delta1 delta2 delta2' : lctx N),
     merge delta1 delta2 delta ->
     merge delta1 delta2' delta ->
